\documentclass{article}
\usepackage[utf8]{inputenc}

\title{T.Bayes}
\author{Atalia Navarro Boullosa }
\date{June 2018}

\begin{document}

\maketitle
Derive Bayes Theorem from $p(x,y) = p(y,x)$ \\
\ \\
Using the probability porperty: $p(x,y) = P(x\mid y)P(y)$ we can write\\
\begin{equation}
   p(x,y) = P(x\mid y)P(y) = P(y\mid x)P(x) = p(y,x)
\end{equation}

\begin{equation}
    P(y\mid x)P(x) = P(x\mid y)P(y)
\end{equation}
Dividing by $P(x)$ in both sides we get

\begin{equation}
    \frac{P(y\mid x)P(x)}{P(x)} = \frac{P(x\mid y)P(y)}{P(x)}
\end{equation}
Finally
\begin{equation}
    P(y\mid x) = \frac{P(x\mid y)P(y)}{P(x)}
\end{equation}
wich is the Bayes Theorem.
\end{document}
